theories/tree_borrows/examples/protected/mutable_reorder_write_up_activated.v
@@ -7,54 +7,49 @@ From simuliris.tree_borrows Require Import proofmode lang adequacy examples.lib.
 From iris.prelude Require Import options.
 
 
+(** Moving a write to a mutable reference up across unknown code. *)
 
-(** Moving read of shared ref up across code that *may* use that ref. *)
-
-(** This is a variant using protectors.
-  See delete_read_pubic_escaped_unprotected.v for the original optimization without protectors and with deferred UB.
- *)
-
-(* Assuming x : & i32 *)
-Definition ex2_unopt : expr :=
+(* Assuming x : &mut i32 *)
+Definition prot_mutable_reorder_write_up_activated_unopt : expr :=
     let: "c" := InitCall in
-
     (* "x" is the local variable that stores the pointer value "i" *)
     let: "x" := new_place sizeof_scalar "i" in
 
     (* retag_place reborrows the pointer value stored in "x" (which is "i"),
-      then updates "x" with the new pointer value.
-      Using a protector here.
-    *)
-    retag_place "x" ShrRef TyFrz sizeof_scalar FnEntry "c";;
+      then updates "x" with the new pointer value. This relies on protectors,
+      hence [FnEntry]. *)
+    retag_place "x" MutRef TyFrz sizeof_scalar FnEntry "c";;
 
-    (* The unknown code is represented by a call to an unknown function "f",
-      which does take the pointer value from "x" as an argument. *)
-    Call #[ScFnPtr "f"] (Copy "x") ;;
+    (* Write 42 to the cell pointed to by the pointer in "x" *)
+    *{sizeof_scalar} "x" <- #[42] ;;
 
-    (* Read the value "v" from the cell pointed to by the pointer in "x" *)
-    let: "v" := Copy *{sizeof_scalar} "x" in
+    (* The unknown code is represented by a call to an unknown function "f" *)
+    let: "v" := Call #[ScFnPtr "f"] #[] in
+
+    (* Write 13 to the cell pointed to by the pointer in "x" *)
+    *{sizeof_scalar} "x" <- #[13] ;;
 
     (* Free the local variable *)
     Free "x" ;;
 
-    (* Finally, return the read value *)
+    (* Finally, return the value *)
     EndCall "c";;
     "v"
   .
 
-Definition ex2_opt : expr :=
+Definition prot_mutable_reorder_write_up_activated_opt : expr :=
     let: "c" := InitCall in
     let: "x" := new_place sizeof_scalar "i" in
-    retag_place "x" ShrRef TyFrz sizeof_scalar FnEntry "c";;
-    let: "v" := Copy *{sizeof_scalar} "x" in
-    Call #[ScFnPtr "f"] (Copy "x") ;;
+    retag_place "x" MutRef TyFrz sizeof_scalar FnEntry "c";;
+    *{sizeof_scalar} "x" <- #[13] ;;
+    let: "v" := Call #[ScFnPtr "f"] #[] in
     Free "x" ;;
     EndCall "c";;
     "v"
   .
 
-Lemma sim_opt2 `{sborGS Σ} :
-  ⊢ log_rel ex2_opt ex2_unopt.
+Lemma prot_mutable_reorder_write_up_activated `{sborGS Σ} :
+  ⊢ log_rel prot_mutable_reorder_write_up_activated_opt prot_mutable_reorder_write_up_activated_unopt.
 Proof.
   log_rel.
   iIntros "%r_t %r_s #Hrel !# %π _".
@@ -82,7 +77,7 @@ Proof.
   iPoseProof (value_rel_singleton_source with "Hv") as (sc_t [= ->]) "Hscrel".
   iPoseProof (sc_rel_ptr_source with "Hscrel") as ([= ->]) "Htagged".
   iApply (sim_retag_fnentry with "Hscrel Hcall"). 1: by cbv.
-  iIntros (t_i v_t v_s _ Hlen_t Hlen_s) "Hcall #Hvrel #Htag_i Hi_t Hi_s".
+  iIntros (t_i v_t v_s _ Hlen_t Hlen_s) "Hcall #Hvrel Htag_i Hi_t Hi_s".
   destruct v_t as [|v_t []]; try done.
   destruct v_s as [|v_s []]; try done. iSimpl in "Hcall".
   iApply sim_expr_base.
@@ -92,39 +87,38 @@ Proof.
   2: done. 1: rewrite /write_range bool_decide_true. 2: simpl; lia. 1: rewrite Z.sub_diag /= //.
   sim_pures.
 
-  (* do the target load *)
-  target_apply (Copy (Place _ _ _)) (target_copy_local with "Htag Ht") "Ht Htag". 2: done.
-  1: rewrite read_range_heaplet_to_list // Z.sub_diag /= //.
-  target_pures. target_bind (Copy _).
-  iApply (target_copy_protected with "Hcall Htag_i Hi_t"). 1: done.
-  2: simpl; lia. 1: rewrite read_range_heaplet_to_list // Z.sub_diag /= //.
-  2: by rewrite lookup_insert.
-  { intros off Hoff. simpl in *. rewrite /range'_contains /sizeof_scalar /= in Hoff. assert (off = i.2)%nat as -> by lia. rewrite /shift_loc /= Z.add_0_r /call_set_in lookup_insert /=. by eexists. }
-  iIntros "Hi_t _ Hcall". target_finish.
-  sim_pures.
-
-  (* do the call *)
-  sim_pures. target_apply (Copy _) (target_copy_local with "Htag Ht") "Ht Htag". 2: done.
-  1: rewrite read_range_heaplet_to_list // Z.sub_diag /= //.
-  source_apply (Copy _) (source_copy_local with "Htag Hs") "Hs Htag". 2: done.
-  1: rewrite read_range_heaplet_to_list // Z.sub_diag /= //. sim_pures.
-  sim_apply (Call _ _) (Call _ _) (sim_call _ (ValR [ScPtr i _]) (ValR [ScPtr i _])) "".
-  { iApply big_sepL2_singleton. iFrame "Htag_i". done. }
-  iIntros (r_t r_s) "_". sim_pures.
-
-  (* do the source load *)
+  (* do the activation write *)
   source_apply (Copy (Place _ _ _)) (source_copy_local with "Htag Hs") "Hs Htag". 2: done.
   1: rewrite read_range_heaplet_to_list // Z.sub_diag /= //.
-  source_pures. source_bind (Copy _).
-  iApply (source_copy_protected with "Hcall Htag_i Hi_s"). 1: done.
-  2: simpl; lia. 1: rewrite read_range_heaplet_to_list // Z.sub_diag /= //.
-  2: by rewrite lookup_insert.
-  { intros off Hoff. simpl in *. rewrite /range'_contains /sizeof_scalar /= in Hoff. assert (off = i.2)%nat as -> by lia. rewrite /shift_loc /= Z.add_0_r /call_set_in lookup_insert /=. by eexists. }
-  iIntros "Hi_s _ Hcall". source_finish.
+  source_pures. source_finish.
+  target_apply (Copy (Place _ _ _)) (target_copy_local with "Htag Ht") "Ht Htag". 2: done.
+  1: rewrite read_range_heaplet_to_list // Z.sub_diag /= //.
+  target_pures.
+
+  sim_apply (Write _ _) (Write _ _) (sim_write_activate_protected with "Htag_i Hi_t Hi_s Hcall") "Htag_i Hi_t Hi_s Hcall". 1-3: done.
+  { intros off Hoff. simpl in *. assert (off = 0)%nat as -> by lia. rewrite /shift_loc /= Z.add_0_r /call_set_in lookup_insert /=. do 2 eexists; split; first done.
+    by rewrite lookup_insert. }
   sim_pures.
+
+  (* arbitrary code *)
+  sim_apply (Call _ _) (Call _ _) (sim_call _ (ValR []) (ValR [])) ""; first by iApply value_rel_empty.
+  iIntros (r_t r_s) "Hsame1". sim_pures.
+
+  (* do the source store *)
+  source_apply (Copy (Place _ _ _)) (source_copy_local with "Htag Hs") "Hs Htag". 2: done.
+  1: rewrite read_range_heaplet_to_list // Z.sub_diag /= //.
+  source_pures. 
+  source_apply (Write (Place _ _ _) _) (source_write_protected_active with "Hcall Htag_i Hi_s") "Hi_s Htag_i Hcall". 1,3,4: done.
+  1: { rewrite write_range_to_to_list; last (simpl; lia). rewrite Z.sub_diag /= //. }
+  2: rewrite lookup_insert //.
+  1: intros off (?&?); assert (off = i.2) as -> by (simpl in *; lia); rewrite /shift_loc /= Z.add_0_r lookup_insert; by eexists.
+  source_pures. source_finish.
 
   (* cleanup: remove the protector ghost state, make the external locations public, free the local locations*)
   sim_apply (Free _) (Free _) (sim_free_local with "Htag Ht Hs") "Htag"; [done..|]. sim_pures.
+  iApply (sim_make_unique_public with "Hi_t Hi_s Htag_i Hcall []"). 1: by rewrite lookup_insert.
+  { iIntros "_". iApply value_rel_int. }
+  iIntros  "Htag_i Hcall". iEval (rewrite !fmap_insert !fmap_empty !insert_insert /=) in "Hcall".
   iApply (sim_protected_unprotect_public with "Hcall Htag_i"). 1: by rewrite lookup_insert.
   iIntros "Hc". iEval (rewrite delete_insert) in "Hc".
   sim_apply (EndCall _) (EndCall _) (sim_endcall_own with "Hc") "".
@@ -132,24 +126,22 @@ Proof.
   sim_val. iModIntro. iSplit; first done. done.
 Qed.
 
-
 Section closed.
   (** Obtain a closed proof of [ctx_ref]. *)
-  Lemma sim_opt2_ctx : ctx_ref ex2_opt ex2_unopt.
+  Lemma prot_mutable_reorder_write_up_activated_ctx : ctx_ref prot_mutable_reorder_write_up_activated_opt prot_mutable_reorder_write_up_activated_unopt.
   Proof.
     set Σ := #[sborΣ].
     apply (log_rel_adequacy Σ)=>?.
-    apply sim_opt2.
+    apply prot_mutable_reorder_write_up_activated.
   Qed.
 End closed.
 
-Check sim_opt2_ctx.
-Print Assumptions sim_opt2_ctx.
+Check prot_mutable_reorder_write_up_activated_ctx.
+Print Assumptions prot_mutable_reorder_write_up_activated_ctx.
 (* 
-sim_opt2_ctx
-     : ctx_ref ex2_opt ex2_unopt
+prot_mutable_reorder_write_up_activated_ctx
+     : ctx_ref prot_mutable_reorder_write_up_activated_opt prot_mutable_reorder_write_up_activated_unopt
 Axioms:
 IndefiniteDescription.constructive_indefinite_description : ∀ (A : Type) (P : A → Prop), (∃ x : A, P x) → {x : A | P x}
 Classical_Prop.classic : ∀ P : Prop, P ∨ ¬ P
 *)
-
